starting closureCLC

CLLean/Completeness/closureCLC.lean
@@ -1,6 +1,6 @@
 /-
 Authors: Kai Obendrauf
-Following the paper "Coalition Logic with Individual, Distributed and Common Knowledge 
+Following the paper "Coalition Logic with Individual, Distributed and Common Knowledge
 by Thomas Ågotnes and Natasha Alechina
 
 This file contains the filtration closure for CLC, and related lemmas
@@ -11,180 +11,196 @@ if ψ ∈ cl φ and subformula χ ψ, then we must have χ ∈ cl φ .
 import CLLean.Syntax.syntaxCLC
 import CLLean.Syntax.propLemmas
 
-local attribute [instance] classical.prop_decidable
-
-open Set formCLC axCLC
+open Classical Set axCLC
 
 ----------------------------------------------------------
 -- Filtration closure cl
 ----------------------------------------------------------
-noncomputable def cl_C {agents : Type} [hN : Fintype agents] (G : Set (agents)) 
+noncomputable def cl_C {agents : Type} [hN : Fintype agents] (G : Set (agents))
   (φ : formCLC agents) : Finset (formCLC agents) :=
-Finset.image (λ i, _K (i) (_C G φ)) (toFinset G) ∪ 
-  Finset.image (λ i, (_¬ _K (i) (_C G φ))) (toFinset G)
+Finset.image (λ i => _K (i) (_C G φ)) (toFinset G) ∪
+  Finset.image (λ i => (_¬ _K (i) (_C G φ))) (toFinset G)
 
-noncomputable def cl {agents : Type} [hN : Fintype agents] : 
+noncomputable def cl {agents : Type} [hN : Fintype agents] :
   formCLC agents → Finset (formCLC agents)
-|  _⊥      := {_⊥, _¬ _⊥}
-| (var n)  := {var n, _¬ (var n), _⊥, _¬ _⊥}
-| (φ _→ ψ) := cl φ ∪ cl ψ ∪ (ite (ψ = _⊥) {(imp φ _⊥)} {(imp φ ψ), _¬ (imp φ ψ)} )
-| (φ _∧ ψ) := cl φ ∪ cl ψ ∪ {(and φ ψ), _¬ (and φ ψ)}
-| ('[G] φ) := cl φ ∪ {('[G] φ), _¬ '[G] φ} ∪ 
-              {(_C (G) ('[G] φ)), _¬ (_C (G) ('[G] φ))} ∪ cl_C G ('[G] φ)
-| (_K i φ) := cl φ ∪ {(_K i φ), _¬ (_K i φ)}
-| (_C G φ) := cl φ ∪ {(_C G φ), _¬ (_C G φ)} ∪ cl_C G φ
+|  _⊥              => {_⊥, _¬ _⊥}
+| (formCLC.var n)  => {formCLC.var n, _¬ (formCLC.var n), _⊥, _¬ _⊥}
+| (φ _→ ψ)         => cl φ ∪ cl ψ ∪ (ite (ψ = _⊥) {(φ _→ _⊥)} {(φ _→ ψ), _¬ (φ _→ ψ)})
+| (φ _∧ ψ)         => cl φ ∪ cl ψ ∪ {(φ _∧ ψ), _¬ (φ _∧ ψ)}
+| (_[G] φ)         => cl φ ∪ {(_[G] φ), _¬ _[G] φ} ∪
+                        {(_C (G) (_[G] φ)), _¬ (_C (G) (_[G] φ))} ∪ cl_C G (_[G] φ)
+| (formCLC.K i φ) => cl φ ∪ {(_K i φ), _¬ (_K i φ)}
+| (_C G φ)        => cl φ ∪ {(_C G φ), _¬ (_C G φ)} ∪ cl_C G φ
 
 ----------------------------------------------------------
 -- Lemmas about cl
 ----------------------------------------------------------
 @[simp] lemma cl_contains_phi {agents : Type} [hN : Fintype agents] (φ : formCLC agents) :
   φ ∈ cl φ := by
-  cases φ
-  repeat { unfold cl, simp, }
-  { split_ifs
-    repeat { simp[h] at *, }, }
+  cases' φ
+  any_goals
+    simp_all only [cl, Finset.union_insert, Finset.mem_union, Finset.mem_insert, Finset.mem_singleton, or_false,
+    eq_self_iff_true, and_self, or_true, true_or, Finset.mem_union, Finset.union_assoc]
+  · unfold cl
+    simp only [Finset.mem_singleton, formCLC.imp.injEq, Finset.union_assoc, Finset.mem_union]
+    split_ifs with h
+    simp only [Finset.mem_singleton, formCLC.imp.injEq, h, and_false, Finset.mem_insert,
+      or_false, or_true]
+    simp only [Finset.mem_singleton, formCLC.imp.injEq, Finset.mem_insert, true_or, or_true]
+
+
 
 @[simp] lemma cl_contains_bot {agents : Type} [hN : Fintype agents] (φ : formCLC agents) :
   _⊥ ∈ cl φ := by
-  induction φ
-  any_goals { unfold cl, simp, }
-  any_goals { simp [φ_ih], }
-  any_goals { simp [φ_ih_φ, φ_ih_ψ], }
+  induction' φ with _ _ _ ih_φ ih_ψ _ _ ih_φ ih_ψ _ _ ih _ _ ih _ _ ih
+  any_goals simp [cl]
+  any_goals simp [ih]
+  any_goals simp [ih_φ, ih_ψ]
 
-lemma cl_C_contains_KC {agents : Type} [hN : Fintype agents] {φ ψ : formCLC agents} 
+lemma cl_C_contains_KC {agents : Type} [hN : Fintype agents] {φ ψ : formCLC agents}
   {G : Set agents} {i : agents} (hi : i ∈ G) (h : _C G ψ ∈ cl φ) : _K i (_C G ψ) ∈ cl φ := by
-  induction φ
-  any_goals 
-  { simp only [cl, Finset.mem_insert, Finset.mem_singleton, or_self] at *, exact h, }
-  { simp only [cl, Finset.mem_insert, Finset.mem_union, Finset.mem_singleton, or_false] at *
-    cases h, exact or.inl (φ_ih_φ h), exact or.inr (φ_ih_ψ h), }
-  { simp only [cl, Finset.union_assoc, Finset.mem_union] at *
-    cases h, exact or.inl (φ_ih_φ h)
-    cases h, simp only [φ_ih_ψ h, true_or, or_true]
-    split_ifs at h, simp only [Finset.mem_singleton] at h, cases h
-    simp only [Finset.mem_insert, Finset.mem_singleton, or_self] at h, cases h, }
-  { simp only [cl, Finset.union_insert, Finset.insert_union, Finset.union_assoc, Finset.mem_insert
-                Finset.mem_union, Finset.mem_singleton, false_or] at *
-    cases h, rw [h.1, h.2] at *
-    simp only [cl_C, hi, Finset.mem_union, Finset.mem_image, mem_to_finset, eq_self_iff_true
+  induction' φ with _ _ _ ih_φ ih_ψ _ _ ih_φ ih_ψ _ _ ih _ _ ih _ _ ih
+  any_goals
+    simp only [cl, Finset.mem_insert, Finset.mem_singleton, or_self] at *
+  · simp only [cl, Finset.mem_insert, Finset.mem_union, Finset.mem_singleton, or_false] at *
+    cases' h with h h
+    · exact Or.inl (ih_φ h)
+    · exact Or.inr (ih_ψ h)
+  · simp only [cl, Finset.union_assoc, Finset.mem_union] at *
+    cases' h with h h
+    · exact Or.inl (ih_φ h)
+    cases' h with h h
+    · simp only [ih_ψ h, true_or, or_true]
+    split_ifs at h
+    · simp only [Finset.mem_singleton] at h
+    · simp only [Finset.mem_insert, Finset.mem_singleton, or_self] at h
+  · simp only [Finset.mem_singleton, Finset.union_insert, Finset.mem_union, or_false,
+    Finset.insert_union, Finset.union_assoc, or_self, Finset.mem_insert, false_or,
+    formCLC.C.injEq] at *
+    cases' h with h h
+    · rw [h.1] at hi
+      simp [h.1, h.2, cl_C, hi, Finset.mem_union, Finset.mem_image, mem_toFinset, eq_self_iff_true,
                 and_true, exists_prop, exists_eq_right, exists_false, or_false, or_true]
-    cases h, exact or.inl (φ_ih h)
-    simp only [cl_C, Finset.mem_union, Finset.mem_image, exists_false, or_false] at h, cases h, }
-  { simp only [cl, Finset.union_insert, Finset.mem_insert, Finset.mem_union, Finset.mem_singleton
-                false_or, or_false] at *
-    exact or.inr (φ_ih h), }
-  { simp only [cl, cl_C, Finset.union_insert, Finset.mem_insert, Finset.mem_union
-                Finset.mem_singleton, Finset.mem_image, mem_to_finset, exists_prop, exists_false
-                or_false, false_or] at *
-    cases h, rw [h.1, h.2] at *
-    simp only [hi, eq_self_iff_true, and_true, exists_eq_right, or_true]
-    exact or.inl (φ_ih h), }
+    cases' h with h h
+    · exact Or.inl (ih h)
+    simp only [cl_C, Finset.mem_union, Finset.mem_image, mem_toFinset, and_false, exists_false,
+      or_self] at h
+  · simp only [Finset.mem_singleton, Finset.union_insert, Finset.mem_union, or_false,
+      Finset.mem_insert, false_or, formCLC.K.injEq] at *
+    exact Or.inr (ih h)
+  · simp only [Finset.mem_singleton, Finset.union_insert, Finset.mem_union, or_false, cl_C,
+      Finset.insert_union, Finset.union_assoc, Finset.mem_image, mem_toFinset, and_false,
+      exists_false, or_self, Finset.mem_insert, formCLC.C.injEq, formCLC.K.injEq, false_or] at *
+    cases' h with h h
+    · rw [h.1] at hi
+      simp only [h.1, h.2, and_true, exists_eq_right, hi, or_true]
+    · exact Or.inl (ih h)
 
-lemma cl_closed_single_neg {agents : Type} [hN : Fintype agents] 
+lemma cl_closed_single_neg {agents : Type} [hN : Fintype agents]
   (φ x : formCLC agents) (hx : x ∈ cl φ) :
   ∃ ψ, (ψ ∈ cl φ ∧ _⊢ (ψ _↔ (_¬ x))) := by
-  induction φ
-  repeat
-    { unfold cl at *
-      simp only [Finset.union_insert, Finset.insert_union, Finset.union_assoc, Finset.mem_insert
+  induction' φ with _ _ _ ih_φ ih_ψ _ _ ih_φ ih_ψ _ _ ih _ _ ih _ _ ih
+  repeat'
+    · unfold cl at *
+      simp only [Finset.union_insert, Finset.insert_union, Finset.union_assoc, Finset.mem_insert,
                   Finset.mem_union, Finset.mem_singleton] at hx
-      cases hx
-      { apply Exists.intro (_¬ x)
+      cases' hx with hx hx
+      · apply Exists.intro (_¬ x)
         simp only [hx, Finset.mem_insert, Finset.mem_union, Finset.mem_singleton, eq_self_iff_true
                     false_or, true_or, or_true, true_and] at *
-        apply @iff_iden (formCLC agents) _ _, }, }
-  { apply Exists.intro (_⊥)
-    simp only [hx, Finset.mem_insert, eq_self_iff_true, Finset.mem_singleton, or_false, true_and]
+        exact iff_iden --apply @iff_iden (formCLC agents) _ _
+  · apply Exists.intro (_⊥)
+    -- simp only [hx, Finset.mem_insert, eq_self_iff_true, Finset.mem_singleton, or_false, true_and]
     apply MP
     apply MP
     apply Prop4
     exact @dni (formCLC agents) _ _
-    exact @nnn_bot (formCLC agents) _, }
-  { cases hx
-   { apply Exists.intro (var φ)
+    exact @nnn_bot (formCLC agents) _
+  · cases hx
+   · apply Exists.intro (var φ)
       simp only [hx, Finset.mem_insert, eq_self_iff_true, Finset.mem_singleton
                   or_false, true_and] at *
-      exact @iff_dni (formCLC agents) _ _, }
+      exact @iff_dni (formCLC agents) _ _
     cases hx
-    { apply Exists.intro ('⊤)
+    · apply Exists.intro ('⊤)
       simp only [hx, Finset.mem_insert, eq_self_iff_true, false_and, Finset.mem_singleton
                   false_or, true_and]
-      apply @iff_iden (formCLC agents) _ _, }
-    { apply Exists.intro (_⊥)
+      apply @iff_iden (formCLC agents) _ _
+    · apply Exists.intro (_⊥)
       simp only [hx, Finset.mem_insert, eq_self_iff_true, Finset.mem_singleton, or_false
                   false_or, true_and]
       apply MP
     apply MP
     apply Prop4
     exact @dni (formCLC agents) _ _
-    exact @nnn_bot (formCLC agents) _, }, }
-  { cases hx
-    { specialize φ_ih_φ hx
+    exact @nnn_bot (formCLC agents) _
+  · cases hx
+    · specialize φ_ih_φ hx
       cases φ_ih_φ with ψ hψ
       apply Exists.intro ψ
       split
       apply Finset.mem_union_left
       apply Finset.mem_union_left
       exact hψ.1
-      exact hψ.2, }
+      exact hψ.2
     cases hx
-    { specialize φ_ih_ψ hx
+    · specialize φ_ih_ψ hx
       cases φ_ih_ψ with ψ hψ
       apply Exists.intro ψ
       split
       apply Finset.mem_union_left
       apply Finset.mem_union_right
       exact hψ.1
-      exact hψ.2, }
-      { apply Exists.intro (φ_φ _∧ φ_ψ)
+      exact hψ.2
+      · apply Exists.intro (φ_φ _∧ φ_ψ)
         simp only [hx, Finset.union_insert, Finset.mem_insert, eq_self_iff_true
                     true_or, true_and]
-        exact @iff_dni (formCLC agents) _ _, }, }
-  { unfold cl at *
+        exact @iff_dni (formCLC agents) _ _
+  · unfold cl at *
     simp only [Finset.union_assoc, Finset.mem_union] at hx
     cases hx
-    { specialize φ_ih_φ hx
+    · specialize φ_ih_φ hx
       cases φ_ih_φ with ψ hψ
       apply Exists.intro ψ
       split
       apply Finset.mem_union_left
       apply Finset.mem_union_left
       exact hψ.1
-      exact hψ.2, }
+      exact hψ.2
     cases hx
-    { specialize φ_ih_ψ hx
+    · specialize φ_ih_ψ hx
       cases φ_ih_ψ with ψ hψ
       apply Exists.intro ψ
       split
       apply Finset.mem_union_left
       apply Finset.mem_union_right
       exact hψ.1
-      exact hψ.2, }
-    { split_ifs at hx
-      { simp only [h, eq_self_iff_true, if_true, Finset.union_assoc, Finset.mem_union
+      exact hψ.2
+    · split_ifs at hx
+      · simp only [h, eq_self_iff_true, if_true, Finset.union_assoc, Finset.mem_union
                     Finset.mem_singleton] at *
         simp only [hx]
         apply Exists.intro (φ_φ)
         split
         apply or.intro_left
         exact cl_contains_phi φ_φ
-        exact @iff_dni (formCLC agents) _ _, }
-      { simp only [h, if_false, Finset.union_insert, Finset.union_assoc, Finset.mem_insert
+        exact @iff_dni (formCLC agents) _ _
+      · simp only [h, if_false, Finset.union_insert, Finset.union_assoc, Finset.mem_insert
                     Finset.mem_union, Finset.mem_singleton, not_false_iff] at *
         cases hx
-        { apply Exists.intro (_¬ (φ_φ _→ φ_ψ))
+        · apply Exists.intro (_¬ (φ_φ _→ φ_ψ))
           simp only [hx, eq_self_iff_true, or_true, true_and]
-          exact @iff_iden (formCLC agents) _ _, }
-        { apply Exists.intro (φ_φ _→ φ_ψ)
+          exact @iff_iden (formCLC agents) _ _
+        · apply Exists.intro (φ_φ _→ φ_ψ)
           simp only [hx, eq_self_iff_true, true_or, true_and]
-          exact @iff_dni (formCLC agents) _ _, }, }, }, }
-  { cases hx
-    {  apply Exists.intro (_¬ (_C φ_G '[φ_G] φ_φ))
+          exact @iff_dni (formCLC agents) _ _
+  · cases hx
+    · apply Exists.intro (_¬ (_C φ_G '[φ_G] φ_φ))
       simp only [hx, Finset.mem_insert, Finset.mem_union, Finset.mem_singleton, eq_self_iff_true
                   true_or, or_true, true_and]
-      exact @iff_iden (formCLC agents) _ _, }
+      exact @iff_iden (formCLC agents) _ _
     cases hx
-    { specialize φ_ih hx
+    · specialize φ_ih hx
       cases φ_ih with ψ hψ
       apply Exists.intro ψ
       split
@@ -192,70 +208,70 @@ lemma cl_closed_single_neg {agents : Type} [hN : Fintype agents]
       apply Finset.mem_union_left
       apply Finset.mem_union_left
       exact hψ.1
-      exact hψ.2, }
+      exact hψ.2
     cases hx
-    { apply Exists.intro ('[φ_G] φ_φ)
+    · apply Exists.intro ('[φ_G] φ_φ)
       simp only [hx, Finset.union_insert, Finset.mem_insert, eq_self_iff_true, Finset.mem_union
                   false_or, true_or, true_and]
-      exact @iff_dni (formCLC agents) _ _, }
+      exact @iff_dni (formCLC agents) _ _
     cases hx
-    { apply Exists.intro (_C φ_G '[φ_G] φ_φ)
+    · apply Exists.intro (_C φ_G '[φ_G] φ_φ)
         simp only [hx, Finset.union_insert, Finset.mem_insert, eq_self_iff_true, Finset.mem_union
                     false_or, true_or, true_and]
-        exact @iff_dni (formCLC agents) _ _, }
-    { unfold cl_C at *
+        exact @iff_dni (formCLC agents) _ _
+    · unfold cl_C at *
       simp only [Finset.mem_union, Finset.mem_image, mem_to_finset, exists_prop] at hx
       cases hx
-      { cases hx with i hi
+      · cases hx with i hi
         apply Exists.intro (_¬ _K i (_C φ_G ('[φ_G]φ_φ)))
         simp only [hi.left, ←hi.right, Finset.mem_union, eq_self_iff_true, Finset.mem_image
                     mem_to_finset, and_true, exists_prop, exists_eq_right, or_true, true_and]
-        exact @iff_iden (formCLC agents) _ _, }
-      { cases hx with i hi
+        exact @iff_iden (formCLC agents) _ _
+      · cases hx with i hi
         apply Exists.intro (_K i (_C φ_G ('[φ_G]φ_φ)))
         simp only [hi.left, ←hi.right, Finset.mem_union, Finset.mem_image, mem_to_finset
                     eq_self_iff_true, and_true, exists_prop, exists_eq_right, exists_false
                     or_false, or_true, true_and]
-        exact @iff_dni (formCLC agents) _ _, }, }, }
-  { cases hx
-    { specialize φ_ih hx
+        exact @iff_dni (formCLC agents) _ _
+  · cases hx
+    · specialize φ_ih hx
       cases φ_ih with ψ hψ
       apply Exists.intro ψ
       split
       apply Finset.mem_union_left
       exact hψ.1
-      exact hψ.2, }
-    { apply Exists.intro (_K φ_a φ_φ)
+      exact hψ.2
+    · apply Exists.intro (_K φ_a φ_φ)
       simp only [hx, Finset.union_insert, Finset.mem_insert, eq_self_iff_true, true_or, true_and]
-      exact @iff_dni (formCLC agents) _ _, }, }
-  { cases hx
-    { specialize φ_ih hx
+      exact @iff_dni (formCLC agents) _ _
+  · cases hx
+    · specialize φ_ih hx
       cases φ_ih with ψ hψ
       apply Exists.intro ψ
       split
       apply Finset.mem_union_left
       apply Finset.mem_union_left
       exact hψ.1
-      exact hψ.2, }
+      exact hψ.2
     cases hx
-    { apply Exists.intro ((_C φ_G (φ_φ)))
+    · apply Exists.intro ((_C φ_G (φ_φ)))
       simp only [hx, Finset.union_insert, Finset.mem_insert, eq_self_iff_true, Finset.mem_union
                   true_or, true_and]
-      exact @iff_dni (formCLC agents) _ _, }
-    { unfold cl_C at *
+      exact @iff_dni (formCLC agents) _ _
+    · unfold cl_C at *
       simp only [Finset.mem_union, Finset.mem_image, mem_to_finset, exists_prop] at hx
       cases hx
-      { cases hx with i hi
+      · cases hx with i hi
         apply Exists.intro (_¬ _K i (_C φ_G φ_φ))
         simp only [hi.left, ←hi.right, Finset.mem_union, eq_self_iff_true, Finset.mem_image
                     mem_to_finset, and_true, exists_prop, exists_eq_right, or_true, true_and]
-        exact @iff_iden (formCLC agents) _ _, }
-      { cases hx with i hi
+        exact @iff_iden (formCLC agents) _ _
+      · cases hx with i hi
         apply Exists.intro (_K i (_C φ_G φ_φ))
         simp only [hi.left, ←hi.right, Finset.mem_union, Finset.mem_image, mem_to_finset
                     eq_self_iff_true, and_true, exists_prop, exists_eq_right, exists_false
                     or_false, or_true, true_and]
-        exact @iff_dni (formCLC agents) _ _, }, }, }
+        exact @iff_dni (formCLC agents) _ _
 
 ----------------------------------------------------------
 -- Subformulas in CLC
@@ -282,7 +298,7 @@ lemma subformula.cl_subset_and_left {agents : Type} [hN : Fintype agents]
   { simp only [cl, Finset.insert_union, Finset.union_insert, Finset.union_assoc, Finset.mem_insert
                 Finset.mem_union, Finset.mem_singleton] at *
     repeat {cases h, simp only [h, eq_self_iff_true, and_self, false_or, true_or, or_true],}
-    {simp only [h, eq_self_iff_true, and_self, true_or, false_or, or_true], }, }
+    {simp only [h, eq_self_iff_true, and_self, true_or, false_or, or_true]
 
 lemma subformula.cl_subset_and_right {agents : Type} [hN : Fintype agents]
   {φ ψ : formCLC agents} : cl ψ ⊆ cl (φ _∧ ψ) := by
@@ -291,7 +307,7 @@ lemma subformula.cl_subset_and_right {agents : Type} [hN : Fintype agents]
   repeat
   { simp [cl] at *
     repeat {cases h, simp [h],}
-    {simp [h], }, }
+    {simp [h]
 
 lemma subformula.cl_subset_imp_left {agents : Type} [hN : Fintype agents]
   {φ ψ : formCLC agents} : cl φ ⊆ cl (φ _→ ψ) := by
@@ -300,7 +316,7 @@ lemma subformula.cl_subset_imp_left {agents : Type} [hN : Fintype agents]
   repeat
   { simp [cl] at *
     repeat {cases h, simp [h],}
-    {simp [h], }, }
+    {simp [h]
 
 lemma subformula.cl_subset_imp_right {agents : Type} [hN : Fintype agents]
   {φ ψ : formCLC agents} : cl ψ ⊆ cl (φ _→ ψ) := by
@@ -309,7 +325,7 @@ lemma subformula.cl_subset_imp_right {agents : Type} [hN : Fintype agents]
   repeat
   { simp [cl] at *
     repeat {cases h, simp [h],}
-    {simp [h], }, }
+    {simp [h]
 
 lemma subformula.cl_subset_effectivity {agents : Type} [hN : Fintype agents]
   {φ : formCLC agents} {G : Set (agents)} : cl φ ⊆ cl ('[G] φ) := by
@@ -318,7 +334,7 @@ lemma subformula.cl_subset_effectivity {agents : Type} [hN : Fintype agents]
   repeat
   { simp [cl] at *
     repeat {cases h, simp [h],}
-    {simp [h], }, }
+    {simp [h]
 
 lemma subformula.cl_subset_knows {agents : Type} [hN : Fintype agents]
   {φ : formCLC agents} {i : agents}  : cl φ ⊆ cl (_K i φ) := by
@@ -327,7 +343,7 @@ lemma subformula.cl_subset_knows {agents : Type} [hN : Fintype agents]
   repeat
   { simp [cl] at *
     repeat {cases h, simp [h],}
-    {simp [h], }, }
+    {simp [h]
 
 lemma subformula.cl_subset_common_know {agents : Type} [hN : Fintype agents]
   {φ : formCLC agents} {G : Set (agents)} : cl φ ⊆ cl (_C G φ) := by
@@ -336,20 +352,20 @@ lemma subformula.cl_subset_common_know {agents : Type} [hN : Fintype agents]
   repeat
   { simp [cl] at *
     repeat {cases h, simp [h],}
-    {simp [h], }, }
+    {simp [h]
 
 lemma subformula.cl_subset {agents : Type} [hN : Fintype agents]
   {φ ψ : formCLC agents} (h : subformula φ ψ) : cl φ ⊆ cl ψ := by
   induction h with _ _ _ _ _ h ih ih'
-  { exact Finset.subset.rfl, }
-  { exact Finset.subset.trans ih ih', }
-  { exact subformula.cl_subset_and_left, }
-  { exact subformula.cl_subset_and_right, }
-  { exact subformula.cl_subset_imp_left, }
-  { exact subformula.cl_subset_imp_right, }
-  { exact subformula.cl_subset_effectivity, }
-  { exact subformula.cl_subset_knows, }
-  { exact subformula.cl_subset_common_know, }
+  { exact Finset.subset.rfl
+  { exact Finset.subset.trans ih ih'
+  { exact subformula.cl_subset_and_left
+  { exact subformula.cl_subset_and_right
+  { exact subformula.cl_subset_imp_left
+  { exact subformula.cl_subset_imp_right
+  { exact subformula.cl_subset_effectivity
+  { exact subformula.cl_subset_knows
+  { exact subformula.cl_subset_common_know
 
 lemma subformula.mem_cl {agents : Type} [hN : Fintype agents]
   {φ ψ : formCLC agents} (h : subformula φ ψ) : φ ∈ cl ψ :=
@@ -358,44 +374,44 @@ h.cl_subset (cl_contains_phi φ)
 lemma subformula.in_cl_sub {agents : Type} [hN : Fintype agents]
   {φ ψ χ : formCLC agents} (hcl : ψ ∈ cl φ) (hsub : subformula χ ψ) : χ ∈ cl φ := by
   induction hsub with _ _ _ _ hsub1 hsub2 hih1 hih2
-  { exact hcl, }
-  { exact hih1 (hih2 hcl), }
+  { exact hcl
+  { exact hih1 (hih2 hcl)
   all_goals
   { induction φ
-    repeat 
+    repeat
     { simp only [cl, Finset.mem_insert, Finset.mem_singleton, or_self] at hcl
-      cases hcl, }, }
+      cases hcl
   any_goals
   { simp only [cl, cl_C, Finset.mem_insert, Finset.mem_union, Finset.mem_singleton
                 Finset.mem_image, exists_false, or_false, false_or] at hcl
-      cases hcl, }
-  repeat { apply or.elim hcl, all_goals { intro hcl, }, }
-  any_goals { split_ifs at hcl, }
-  any_goals { rw hcl.1 at *, rw hcl.2 at *, }
-  any_goals { rw h at *, }
+      cases hcl
+  repeat { apply or.elim hcl, all_goals { intro hcl
+  any_goals { split_ifs at hcl
+  any_goals { rw hcl.1 at *, rw hcl.2 at *
+  any_goals { rw h at *
   any_goals { simp only [cl, Finset.union_assoc, Finset.mem_insert, Finset.mem_union
                           Finset.mem_singleton, false_or, Finset.mem_insert, Finset.mem_singleton
                           or_self, or_false, eq_self_iff_true, and_self, or_true
-                          true_or] at hcl, }
+                          true_or] at hcl
   any_goals { simp only [cl_C, Finset.mem_union, Finset.mem_image, exists_false, or_self
-                          or_false] at hcl, }
-  repeat { apply or.elim hcl, all_goals { intro hcl, }, }
-  any_goals { rw hcl.1 at *, rw hcl.2 at *, }
-  any_goals { rw h at *, }
-  any_goals { solve1 { by_contra, exact hcl, }, }
-  any_goals { simp only [cl, φ_ih_φ hcl, Finset.mem_union, true_or, or_true], }
-  any_goals { simp only [cl, φ_ih_ψ hcl, Finset.mem_union, true_or, or_true], }
-  any_goals { simp only [cl, Finset.mem_union, cl_contains_phi, true_or, or_true], }
-  any_goals { simp only [φ_ih hcl, true_or], }
+                          or_false] at hcl
+  repeat { apply or.elim hcl, all_goals { intro hcl
+  any_goals { rw hcl.1 at *, rw hcl.2 at *
+  any_goals { rw h at *
+  any_goals { solve1 { by_contra, exact hcl
+  any_goals { simp only [cl, φ_ih_φ hcl, Finset.mem_union, true_or, or_true]
+  any_goals { simp only [cl, φ_ih_ψ hcl, Finset.mem_union, true_or, or_true]
+  any_goals { simp only [cl, Finset.mem_union, cl_contains_phi, true_or, or_true]
+  any_goals { simp only [φ_ih hcl, true_or]
   any_goals { simp only [if_true, Finset.mem_insert, Finset.mem_singleton, or_false
-                          eq_self_iff_true, and_self, or_true, true_or], }
+                          eq_self_iff_true, and_self, or_true, true_or]
   any_goals { simp only [hcl.1, hcl.2, eq_self_iff_true, cl_contains_phi, and_self
-                          or_false, or_true, true_or], }
+                          or_false, or_true, true_or]
   any_goals { simp only [h, if_false, Finset.mem_insert, eq_self_iff_true, and_self
-                          Finset.mem_singleton, and_false, or_false, or_true], }
+                          Finset.mem_singleton, and_false, or_false, or_true]
   any_goals { obtain ⟨i, ⟨hi, hcl⟩⟩ := hcl
               rw ←hcl.1 at *, rw ←hcl.2 at *
               simp only [cl_C, or_false, Finset.mem_union, Finset.mem_image, mem_to_finset
                           eq_self_iff_true, and_true, exists_prop, exists_eq_right, exists_false
-                          mem_to_finset.mp hi, or_true], }
-  any_goals { simp only [cl_contains_bot, or_self, true_or], }
+                          mem_to_finset.mp hi, or_true]
+  any_goals { simp only [cl_contains_bot, or_self, true_or]
